src/Lean/Meta/ArgsPacker.lean
@@ -486,7 +486,7 @@ Given types `(x : A) → (y : B[x]) → R₁[x,y]` and `(z : C) → R₂[z]`, re
 ```
 -/
 def uncurryType (argsPacker : ArgsPacker) (types : Array Expr) : MetaM Expr := do
-  let unary ← (Array.zipWith Unary.uncurryType argsPacker.varNamess types).mapM id
+  let unary ← Array.zipWithM Unary.uncurryType argsPacker.varNamess types
   Mutual.uncurryType unary
 
 /--
@@ -497,11 +497,11 @@ and `(z : C) → R₂[z]`, returns an expression of type
 ```
 -/
 def uncurry (argsPacker : ArgsPacker) (es : Array Expr) : MetaM Expr := do
-  let unary ← (Array.zipWith Unary.uncurry argsPacker.varNamess es).mapM id
+  let unary ← Array.zipWithM Unary.uncurry argsPacker.varNamess es
   Mutual.uncurry unary
 
 def uncurryWithType (argsPacker : ArgsPacker) (resultType : Expr) (es : Array Expr) : MetaM Expr := do
-  let unary ← (Array.zipWith Unary.uncurry argsPacker.varNamess es).mapM id
+  let unary ← Array.zipWithM Unary.uncurry argsPacker.varNamess es
   Mutual.uncurryWithType resultType unary
 
 /--
@@ -512,7 +512,7 @@ and `(z : C) → R`, returns an expression of type
 ```
 -/
 def uncurryND (argsPacker : ArgsPacker) (es : Array Expr) : MetaM Expr := do
-  let unary ← (Array.zipWith Unary.uncurry argsPacker.varNamess es).mapM id
+  let unary ← Array.zipWithM Unary.uncurry argsPacker.varNamess es
   Mutual.uncurryND unary
 
 /--
@@ -548,7 +548,7 @@ Given type `(x : a ⊗' b ⊕' c ⊗' d) → R` (dependent), return types
 -/
 def curryType (argsPacker : ArgsPacker) (t : Expr) : MetaM (Array Expr) := do
   let unary ← Mutual.curryType argsPacker.numFuncs t
-  (Array.zipWith Unary.curryType argsPacker.varNamess unary).mapM id
+  Array.zipWithM Unary.curryType argsPacker.varNamess unary
 
 /--
 Given expression `e` of type `(x : a ⊗' b ⊕' c ⊗' d) → e[x]`, wraps that expression
